src/program_proof/wal/write_proof.v
@@ -419,19 +419,6 @@ Proof.
   rewrite memWrite_same_start //.
 Qed.
 
-Lemma subslice_from_take {A} m (l: list A) :
-  take m l = subslice 0 m l.
-Proof.
-  rewrite /subslice //.
-Qed.
-
-Lemma subslice_from_drop {A} n (l: list A) :
-  drop n l = subslice n (length l) l.
-Proof.
-  rewrite /subslice.
-  rewrite take_ge; auto.
-Qed.
-
 Lemma memWrite_one_endPos σ u :
   slidingM.wf σ ->
   slidingM.memEnd σ + 1 < 2 ^ 64 ->
